some more dafny

Dafny/cleanup3/Blood.dfy
@@ -7,6 +7,7 @@ class Blood
     var donorName: string;
     var dateDonated: int;
     var locationAcquired: string;
+    var tested: bool;
     
     predicate Valid()
         reads this;
@@ -14,7 +15,8 @@ class Blood
         validBloodType(bloodType)
     }
 
-    constructor(bloodType: BloodType, donorName: string, dateDonated: int, locationAcquired: string)
+    constructor(bloodType: BloodType, donorName: string, dateDonated: int,
+                locationAcquired: string, tested: bool)
         modifies this;
         requires validBloodType(bloodType);
         ensures  Valid();
@@ -22,11 +24,13 @@ class Blood
         ensures  this.donorName == donorName;
         ensures  this.dateDonated == dateDonated;
         ensures  this.locationAcquired == locationAcquired;
+        ensures  this.tested == tested;
     {
         this.bloodType := bloodType;
         this.donorName := donorName;
         this.dateDonated := dateDonated;
         this.locationAcquired := locationAcquired;
+        this.tested := tested;
     }
 
     function method GetBloodType(): BloodType
@@ -53,6 +57,12 @@ class Blood
         locationAcquired
     }
 
+    function method HasBeenTested(): bool
+        reads this;
+    {
+        tested
+    }
+
     predicate method IsExpired(currentDate: int)
         reads this;
     {
@@ -65,20 +75,51 @@ class Blood
     {
         print "Blood from:  ",     donorName,   "\n",
               "Received on: Day ", dateDonated, "\n",
-              "Blood type:  ",     bloodType,   "\n";
+              "Blood type:  ",     bloodType,   "\n",
+              "Tested:      ",     tested,      "\n";
     }
 
 } // end of Blood class
 
+////////////////////////////////////////////////////////////////////////////////
+
+method PrintBloodArray(a: array<Blood>)
+    requires a != null;
+    requires forall i | 0 <= i < a.Length ::
+                        a[i] != null &&
+                        a[i].Valid();
+{
+    print "===============================\n";
+
+    var i := 0;
+    while i < a.Length
+    {
+        a[i].PrettyPrint();
+        if i < a.Length - 1
+        {
+            print "-------------------------------\n";
+        }
+        i := i + 1;
+    }
+
+    print "===============================\n";
+}
+
+////////////////////////////////////////////////////////////////////////////////
+
+// method Main()
+// {
+//     TestBlood();
+// }
+
 method TestBlood()
 {
-    var bobsBlood := new Blood(AM, "Bob", 12, "Prince of Wales Hospital");
+    var blood := new Blood(AM, "Bob", 12, "Prince of Wales Hospital", true);
     
-    assert bobsBlood.GetBloodType() == AM;
-    assert bobsBlood.GetDonorName() == "Bob";
-    assert bobsBlood.GetDateDonated() == 12;
-    bobsBlood.PrettyPrint();
-
-    assert bobsBlood.GetBloodType() == AM;
-    assert bobsBlood.GetBloodType() != AP;
+    assert blood.GetBloodType()   == AM;
+    assert blood.GetBloodType()   != AP;
+    assert blood.GetDonorName()   == "Bob";
+    assert blood.GetDateDonated() == 12;
+    assert blood.HasBeenTested()  == true;
+    blood.PrettyPrint();
 }
