Dafny/cleanup3/SortBloodByDate.dfy
@@ -1,0 +1,196 @@
+/* SortBloodByDate.dfy
+ *
+ * Merge sorts an array of Blood objects by date donated
+ */
+
+include "Blood.dfy"
+
+method Main()
+{
+    var a := new Blood[3];
+    var b1 := new Blood(AP, "Amy", 21, "Hospital", true);
+    var b2 := new Blood(OM, "Bob",  8, "Hospital", true);
+    var b3 := new Blood(AM, "Cal", 13, "Hospital", true);
+    
+    a[0], a[1], a[2] := b1, b2, b3;
+    assert a[..] == [b1, b2, b3];
+    print "Original:\n";
+    PrintBloodArray(a);
+    SortBloodByDate(a);
+    print "Sorted:\n";
+    assert a[..] == [b2, b3, b1];
+    PrintBloodArray(a);
+}
+
+method SortBloodByDate(a: array<Blood>)
+    modifies a;
+    requires a != null;
+    requires forall i | 0 <= i < a.Length ::
+                        a[i] != null &&
+                        a[i].Valid();
+    ensures  forall i | 0 <= i < a.Length ::
+                        a[i] != null &&
+                        a[i].Valid();
+    ensures  sorted(a);
+    ensures  permutation(a[..], old(a[..]));
+{
+    MergeSort(a);
+}
+
+method MergeSort(a: array<Blood>)
+    modifies a;
+    requires a != null;
+    requires forall i | 0 <= i < a.Length ::
+                        a[i] != null &&
+                        a[i].Valid();
+    ensures  forall i | 0 <= i < a.Length ::
+                        a[i] != null &&
+                        a[i].Valid();
+    ensures  sorted(a);
+    ensures  permutation(a[..], old(a[..]));
+{
+    if a.Length == 0 {
+        return;
+    }
+
+    DoMergeSort(a, 0, a.Length);
+
+    assert a[..] == a[0..a.Length];
+    assert old(a[..]) == old(a[0..a.Length]);
+}
+
+method DoMergeSort(a: array<Blood>, l: int, r: int)
+    modifies  a;
+    requires  a != null;
+    requires  forall i | 0 <= i < a.Length ::
+                         a[i] != null &&
+                         a[i].Valid();
+    requires  0 <= l < r <= a.Length;
+    ensures   forall i | 0 <= i < a.Length ::
+                         a[i] != null &&
+                         a[i].Valid();
+    ensures   sortedFromTo(a, l, r);
+    ensures   permutation(a[l..r], old(a[l..r]));
+    ensures   a[..l] == old(a[..l]);
+    ensures   a[r..] == old(a[r..]);
+    decreases r - l;
+{
+    if l == r - 1 {
+        return;
+    }
+
+    var m := (l + r) / 2;
+
+    DoMergeSort(a, l, m);
+    assert sortedFromTo(a, l, m); // subarray from l to m sorted
+    assert permutation(a[l..m], old(a[l..m]));
+    assert a[m..r] == old(a[m..r]); // subarray from m to r unchanged
+
+    DoMergeSort(a, m, r);
+
+    assert a[l..m] + a[m..r] == a[l..r];
+    assert old(a[l..m]) + old(a[m..r]) == old(a[l..r]);
+
+    Merge(a, l, m, r);
+}
+
+method Merge(a: array<Blood>, l: int, m: int, r: int)
+    modifies a;
+    requires a != null;
+    requires forall i | 0 <= i < a.Length ::
+                        a[i] != null &&
+                        a[i].Valid();
+    requires 0 <= l < m < r <= a.Length;
+    requires sortedFromTo(a, l, m);
+    requires sortedFromTo(a, m, r);
+    ensures  forall i | 0 <= i < a.Length ::
+                        a[i] != null &&
+                        a[i].Valid();
+    ensures  sortedFromTo(a, l, r);
+    ensures  permutation(a[l..r], old(a[l..r]));
+    ensures  a[..l] == old(a[..l]);
+    ensures  a[r..] == old(a[r..]);
+{
+    var b := new Blood[a.Length];
+    var i := l;
+    var j := m;
+    var k := l;
+
+    while i < m || j < r
+        decreases m - i + r - j;
+        invariant l <= i <= m && m <= j <= r;
+        invariant k == l + (i - l) + (j - m);
+        invariant a[..] == old(a[..]);
+        invariant forall x | 0 <= x < a.Length ::
+                             a[x] != null &&
+                             a[x].Valid();
+        invariant forall x | l <= x < k ::
+                             b[x] != null &&
+                             b[x].Valid();
+        invariant sortedFromTo(b, l, k);
+        invariant k > l && i < m ==> dateDonatedLe(b[k - 1], a[i]);
+        invariant k > l && j < r ==> dateDonatedLe(b[k - 1], a[j]);
+        invariant permutation(b[l..k], a[l..i] + a[m..j]);
+    {
+        if i == m {
+            b[k] := a[j];
+            j := j + 1;
+        } else if j == r {
+            b[k] := a[i];
+            i := i + 1;
+        } else if dateDonatedLe(a[i], a[j]) {
+            b[k] := a[i];
+            i := i + 1;
+        } else {
+            b[k] := a[j];
+            j := j + 1;
+        }
+        k := k + 1;
+    }
+
+    assert a[l..r] == a[l..m] + a[m..r];
+
+    forall i | l <= i < r
+    {
+        a[i] := b[i];
+    }
+
+    assert a[l..r] == b[l..r];
+}
+
+predicate sorted(a: array<Blood>)
+    reads a;
+    reads set i | 0 <= i < a.Length :: a[i];
+    requires a != null;
+    requires forall i | 0 <= i < a.Length ::
+                        a[i] != null &&
+                        a[i].Valid();
+{
+    sortedFromTo(a, 0, a.Length)
+}
+
+predicate sortedFromTo(a: array<Blood>, l: int, r: int)
+    reads a;
+    reads set i | 0 <= i < a.Length :: a[i];
+    requires a != null;
+    requires 0 <= l <= r <= a.Length;
+    requires forall i | l <= i < r ::
+                        a[i] != null &&
+                        a[i].Valid();
+{
+    forall i, j :: l <= i < j < r ==> dateDonatedLe(a[i], a[j])
+}
+
+predicate method dateDonatedLe(a: Blood, b: Blood)
+    reads a;
+    reads b;
+    requires a != null && a.Valid();
+    requires b != null && b.Valid();
+{
+    a.GetDateDonated() <= b.GetDateDonated()
+}
+
+predicate permutation(a: seq<Blood>, b: seq<Blood>)
+{
+    multiset(a) == multiset(b)
+}
